trying to prove termination mgu

mgu.fst
@@ -27,49 +27,53 @@ let rec collate l1 l2 = match l1,l2 with
 
 let rec is_Unifiable*)
 
-val sub_comp: term -> Tot nat
-val sub_comp_list : list term -> Tot nat
+val sub_comp : lt:list term -> Tot nat
 
-let rec sub_comp t = match t with
-  | Var v -> 1
-  | Name n -> 1
-  | Func s args -> 1 + sub_comp_list args
-and sub_comp_list args = match args with
-  | [] -> 0
-  | hd::tl -> sub_comp hd + sub_comp_list tl
+let rec sub_comp lt = 
 
-val complexity : list (term*term) -> Tot nat
+val get_num_vars : lt:list term -> list variable -> Tot nat (decreases sub_comp lt)
 
-let rec complexity l = match l with
-  | [] -> 0
-  | hd::tl -> (sub_comp (fst hd)) + (sub_comp (snd hd)) + complexity tl
+let rec get_num_vars lt lv =
+  match lt with
+  | (Var v)::tl -> if mem v lv then get_num_vars tl lv else get_num_vars tl (v::lv)
+  | (Name n)::tl -> get_num_vars tl lv
+  | (Func s args)::tl -> get_num_vars (List.Tot.append args tl) lv
 
-val sub_mgu : l:list (term*term) -> st:subst -> Tot (option subst)
+val get_num_symbols : lt:list term -> Tot nat (decreases sub_comp lt)
+
+let rec get_num_symbols lt =
+  match lt with
+  | (Var v)::tl -> 1 + get_num_symbols tl
+  | (Name n)::tl -> 1 + get_num_symbols tl
+  | (Func s args)::tl -> 1 + get_num_symbols (List.Tot.append args tl)
+
+val sub_mgu : l:list (term*term) -> st:subst -> Tot (option subst) (decreases %[(get_num_vars l []);(get_num_symbols l)])
 let rec sub_mgu l st = match l with
   | [] -> Some st
   | (Var v, x)::tl -> begin
-                        if not(isnt_cyclic [(v,x)]) then None
+                        if (is_var_present v x) then None
                         else (
                           let temp1 = (compose st [(v,x)]) in
                           let temp2 = (apply_tuple_list [(v,x)] tl) in
                           apply_list_length_lemma [(v,x)] tl;
-                          (assert (complexity temp2 < complexity l));
+                          (assert (temp2 << l));
                           if None? (sub_mgu temp2 temp1) then None
                           else (sub_mgu temp2 temp1)
                         )
                       end
   | (x,Var v)::tl -> begin
-                        if not(isnt_cyclic [(v,x)]) then None
+                        if (is_var_present v x) then None
                         else (
                           let temp1 = (compose st [(v,x)]) in
                           let temp2 = (apply_tuple_list [(v,x)] tl) in
                           apply_list_length_lemma [(v,x)] tl;
-                          (assert (complexity temp2 < complexity l));
+                          (*(assert (complexity temp2 < complexity l));*)
                           if None? (sub_mgu temp2 temp1) then None
                           else (sub_mgu temp2 temp1)
                         )
                      end
   | (Func s args1, Func s args2)::tl -> sub_mgu (List.Tot.append (collate args1 args2) tl) st
+  | (Name a, Name a)::tl  -> sub_mgu tl st
   | _ -> None
 
 val mgu : l:list (term*term) -> Tot (option subst)
